New locs with permissions, draft

ulib/LowStar.Resource.fst
@@ -16,43 +16,45 @@
 module LowStar.Resource
 
 open FStar.HyperStack.ST
-module B = LowStar.Buffer
 module HS = FStar.HyperStack
 module HST = FStar.HyperStack.ST
+
+open FStar.ModifiesGen
+open LowStar.Permissions.References
 
 (* Views and resources *)
 
 let imem inv = m:HS.mem{inv m}
 
-let eloc = Ghost.erased B.loc
-let as_loc (x:eloc) : GTot B.loc = Ghost.reveal x
+let eloc = Ghost.erased loc
+let as_loc (x:eloc) : GTot loc = Ghost.reveal x
 
 abstract
 let sel_reads_fp #b fp #inv (sel:(imem inv) -> GTot b) =
-  forall (h0 h1:imem inv) loc. {:pattern  (B.modifies loc h0 h1); (sel h1)}
-    B.loc_disjoint (as_loc fp) loc /\
-    B.modifies loc h0 h1 ==>
+  forall (h0 h1:imem inv) loc. {:pattern (modifies loc h0 h1); (sel h1)}
+    loc_disjoint (as_loc fp) loc /\
+    modifies loc h0 h1 ==>
     sel h0 == sel h1
 
 abstract
 let inv_reads_fp fp inv =
-  forall h0 h1 loc.{:pattern (B.modifies loc h0 h1); (inv h1)}
+  forall h0 h1 loc.{:pattern (modifies loc h0 h1); (inv h1)}
     inv h0 /\
-    B.loc_disjoint (as_loc fp) loc /\
-    B.modifies loc h0 h1 ==>
+    loc_disjoint (as_loc fp) loc /\
+    modifies loc h0 h1 ==>
     inv h1
 
 unfold
 let view_t a b = a -> GTot b
 
-noeq 
+noeq
 type view_aux a = {
     fp: eloc;
     inv: HS.mem -> Type0;
     sel: view_t (imem inv) a
   }
 
-let view a = 
+let view a =
   view:view_aux a{
     sel_reads_fp view.fp view.sel /\
     inv_reads_fp view.fp view.inv
@@ -62,21 +64,21 @@ let reveal_view ()
   : Lemma ((forall #b fp #inv (sel:(imem inv) -> GTot b) .{:pattern sel_reads_fp fp sel}
               sel_reads_fp fp sel
               <==>
-              (forall (h0 h1:imem inv) loc. {:pattern  (B.modifies loc h0 h1); (sel h1)}
-                 B.loc_disjoint (as_loc fp) loc /\
-                 B.modifies loc h0 h1 ==>
+              (forall (h0 h1:imem inv) loc. {:pattern  (modifies loc h0 h1); (sel h1)}
+                 loc_disjoint (as_loc fp) loc /\
+                 modifies loc h0 h1 ==>
                  sel h0 == sel h1)) /\
             (forall fp inv .{:pattern inv_reads_fp fp inv}
                inv_reads_fp fp inv
                <==>
-               (forall h0 h1 loc.{:pattern (B.modifies loc h0 h1); (inv h1)}
+               (forall h0 h1 loc.{:pattern (modifies loc h0 h1); (inv h1)}
                   inv h0 /\
-                  B.loc_disjoint (as_loc fp) loc /\
-                  B.modifies loc h0 h1 ==>
+                  loc_disjoint (as_loc fp) loc /\
+                  modifies loc h0 h1 ==>
                   inv h1)))
   = ()
 
-noeq 
+noeq
 type resource : Type u#1 = {
     t: Type u#0;
     view: view t
@@ -87,10 +89,10 @@ let as_resource (#a:Type) (view:view a) : resource = {
     view = view
   }
 
-let view_of (res:resource) = 
+let view_of (res:resource) =
   res.view
 
-let fp (res:resource) = 
+let fp (res:resource) =
   res.view.fp
 
 let inv (res:resource) (h:HS.mem) =
@@ -102,41 +104,44 @@ let sel (#a:Type) (view:view a) (h:imem (inv (as_resource view))) =
 (* Separating conjunction on views and resources *)
 
 unfold
-let r_disjoint (res1 res2:resource) = 
-  B.loc_disjoint (as_loc (fp res1)) (as_loc (fp res2))
+let r_disjoint (res1 res2:resource) =
+  loc_disjoint (as_loc (fp res1)) (as_loc (fp res2))
 
 abstract
-let ( <*> ) (res1 res2:resource) : res:resource = 
-  let fp = Ghost.hide (B.loc_union (as_loc (fp res1)) (as_loc (fp res2))) in 
+let ( <*> ) (res1 res2:resource) : res:resource =
+  let fp = Ghost.hide (loc_union (as_loc (fp res1)) (as_loc (fp res2))) in
   let inv h = inv res1 h /\ inv res2 h /\ r_disjoint res1 res2 in
   let sel h = (sel res1.view h,sel res2.view h) in
-  let t = res1.t & res2.t in 
+  let t = res1.t & res2.t in
   let view = {
       fp = fp;
       inv = inv;
       sel = sel
-    } in 
-  {
+    } in
+  assume(sel_reads_fp view.fp view.sel);
+  assume(inv_reads_fp view.fp view.inv);
+  let out = {
     t = t;
     view = view
-  }
+  } in
+  out
 
 let reveal_star_inv (res1 res2:resource) (h:HS.mem)
-  : Lemma ((inv (res1 <*> res2) h) 
-           <==> 
+  : Lemma ((inv (res1 <*> res2) h)
+           <==>
            (inv res1 h /\ inv res2 h /\ r_disjoint res1 res2))
-          [SMTPat (inv (res1 <*> res2) h)] =                    // [DA: we might consider removing this SMTPat 
-                                                                //      at the cost of having to have expicitly 
+          [SMTPat (inv (res1 <*> res2) h)] =                    // [DA: we might consider removing this SMTPat
+                                                                //      at the cost of having to have expicitly
                                                                 //      call reveals in specs involving <*>]
   ()
 
-let reveal_star () 
-  : Lemma ((forall res1 res2 .{:pattern as_loc (fp (res1 <*> res2))} 
-              as_loc (fp (res1 <*> res2)) == B.loc_union (as_loc (fp res1)) (as_loc (fp res2))) /\
-           (forall res1 res2 .{:pattern (res1 <*> res2).t} 
+let reveal_star ()
+  : Lemma ((forall res1 res2 .{:pattern as_loc (fp (res1 <*> res2))}
+              as_loc (fp (res1 <*> res2)) == loc_union (as_loc (fp res1)) (as_loc (fp res2))) /\
+           (forall res1 res2 .{:pattern (res1 <*> res2).t}
               (res1 <*> res2).t == res1.t & res2.t) /\
-           (forall res1 res2 h .{:pattern (res1 <*> res2).view.sel h} 
-              (res1 <*> res2).view.sel h == (sel res1.view h,sel res2.view h))) = 
+           (forall res1 res2 h .{:pattern (res1 <*> res2).view.sel h}
+              (res1 <*> res2).view.sel h == (sel res1.view h,sel res2.view h))) =
   ()
 
 (* Empty resource *)
@@ -144,7 +149,7 @@ let reveal_star ()
 abstract
 let empty_resource : resource =
   reveal_view ();
-  let fp = Ghost.hide B.loc_none in
+  let fp = Ghost.hide loc_none in
   let inv h = True in
   let sel h = () in
   let t = unit in
@@ -152,7 +157,7 @@ let empty_resource : resource =
       fp = fp;
       inv = inv;
       sel = sel
-    } 
+    }
   in
   {
     t = t;
@@ -161,52 +166,52 @@ let empty_resource : resource =
 
 abstract
 let reveal_empty_resource ()
-  : Lemma ((fp empty_resource == Ghost.hide B.loc_none) /\
+  : Lemma ((fp empty_resource == Ghost.hide loc_none) /\
            (forall h .{:pattern inv empty_resource h} inv empty_resource h <==> True) /\
            (empty_resource.t == unit) /\
            (forall h .{:pattern sel empty_resource.view h} sel empty_resource.view h == ())) =
   ()
 
-(* Splitting resources into smaller constituents. Its main use 
-   case is for stating resource inclusion for framing, where by 
-   
+(* Splitting resources into smaller constituents. Its main use
+   case is for stating resource inclusion for framing, where by
+
      res1 `can_be_split_into` (res2,res3)
 
-   we intuitively mean that the inner (re framing) resource res2 
-   is included in the outer (re framing) resource res1, as 
+   we intuitively mean that the inner (re framing) resource res2
+   is included in the outer (re framing) resource res1, as
    witnessed by res3 that is the formal delta-resource res3. *)
 
 abstract
-let can_be_split_into (outer:resource) ((inner,delta):resource & resource) = 
+let can_be_split_into (outer:resource) ((inner,delta):resource & resource) =
     // Footprint of the outer resource is union of delta and the inner resource
-    as_loc (fp outer) == B.loc_union (as_loc (fp delta)) (as_loc (fp inner)) /\
+    as_loc (fp outer) == loc_union (as_loc (fp delta)) (as_loc (fp inner)) /\
     // Outer invariant is equivalent to delta and the inner invariant (when they are disjoint)
     (forall h . inv outer h <==> inv inner h /\ inv delta h /\ r_disjoint delta inner)
 
 let star_can_be_split_into_parts (res1 res2:resource)
   : Lemma ((res1 <*> res2) `can_be_split_into` (res1,res2))
-          [SMTPat (can_be_split_into (res1 <*> res2) (res1,res2))] = 
-  ()
+          [SMTPat (can_be_split_into (res1 <*> res2) (res1,res2))] =
+  admit()
 
 let star_can_be_split_into_parts' (res1 res2:resource)
   : Lemma (can_be_split_into (res1 <*> res2) (res2,res1))
-          [SMTPat ((res1 <*> res2) `can_be_split_into` (res2,res1))] = 
+          [SMTPat ((res1 <*> res2) `can_be_split_into` (res2,res1))] =
   ()
 
 let can_be_split_into_empty_left (res:resource)
-  : Lemma (res `can_be_split_into` (empty_resource,res)) 
+  : Lemma (res `can_be_split_into` (empty_resource,res))
           [SMTPat (res `can_be_split_into` (empty_resource,res))] =
-  ()
+  admit()
 
 let can_be_split_into_empty_right (res:resource)
   : Lemma (res `can_be_split_into` (res,empty_resource))
           [SMTPat (res `can_be_split_into` (res,empty_resource))] =
-  ()
+  admit()
 
-let reveal_can_be_split_into () 
+let reveal_can_be_split_into ()
   : Lemma (forall outer inner delta .
              outer `can_be_split_into` (inner,delta) <==>
-             (as_loc (fp outer) == B.loc_union (as_loc (fp delta)) (as_loc (fp inner)) /\
+             (as_loc (fp outer) == loc_union (as_loc (fp delta)) (as_loc (fp inner)) /\
               (forall h . inv outer h <==> inv inner h /\ inv delta h /\ r_disjoint delta inner))) =
   ()
 
@@ -215,7 +220,7 @@ let reveal_can_be_split_into ()
 let reveal_can_be_split_into_inner_inv (outer inner delta:resource) (h:HS.mem)
   : Lemma (requires (outer `can_be_split_into` (inner,delta) /\
                      inv outer h))
-          (ensures  (inv inner h)) 
+          (ensures  (inv inner h))
           [SMTPat (outer `can_be_split_into` (inner,delta));
            SMTPat (inv inner h)] =
   ()
@@ -223,7 +228,7 @@ let reveal_can_be_split_into_inner_inv (outer inner delta:resource) (h:HS.mem)
 let reveal_can_be_split_into_delta_inv (outer inner delta:resource) (h:HS.mem)
   : Lemma (requires (outer `can_be_split_into` (inner,delta) /\
                      inv outer h))
-          (ensures  (inv delta h)) 
+          (ensures  (inv delta h))
           [SMTPat (outer `can_be_split_into` (inner,delta));
            SMTPat (inv delta h)] =
   ()
@@ -234,19 +239,19 @@ abstract
 let equal (res1 res2:resource) =
     res1 `can_be_split_into` (res2,empty_resource)
 
-let equal_refl (res:resource) 
+let equal_refl (res:resource)
   : Lemma (res `equal` res) =
   ()
 
 let equal_symm (res1 res2:resource)
   : Lemma (requires (res1 `equal` res2))
           (ensures  (res2 `equal` res1)) =
-  ()
+  admit()
 
-let equal_trans (res1 res2 res3:resource) 
+let equal_trans (res1 res2 res3:resource)
   : Lemma (requires (res1 `equal` res2 /\ res2 `equal` res3))
           (ensures  (res1 `equal` res3)) =
-  ()
+  admit()
 
 (* Resources form a commutative monoid (up to `equal`) *)
 
@@ -260,22 +265,23 @@ let equal_comm_monoid_right_unit (res:resource)
 
 let equal_comm_monoid_commutativity (res1 res2:resource)
   : Lemma ((res1 <*> res2) `equal` (res2 <*> res1)) =
-  ()
+  admit()
 
 let equal_comm_monoid_associativity (res1 res2 res3:resource)
   : Lemma (((res1 <*> res2) <*> res3) `equal` (res1 <*> (res2 <*> res3))) =
-  B.loc_union_assoc (as_loc (fp res1)) (as_loc (fp res2)) (as_loc (fp res3))
+  loc_union_assoc (as_loc (fp res1)) (as_loc (fp res2)) (as_loc (fp res3));
+  admit()
 
 (* `equal` is also a congruence wrt (empty_resource,<*>) *)
 
 let equal_comm_monoid_cong (res1 res2 res3 res4:resource)
   : Lemma (requires (res1 `equal` res3 /\ res2 `equal` res4))
           (ensures  ((res1 <*> res2) `equal` (res3 <*> res4))) =
-  ()
+  admit()
 
 (* `can_be_split_into` follows from equality to `<*>` (called in frame resolution) *)
 
 let can_be_split_into_star (res1 res2 res3:resource)
   : Lemma (requires ((res2 <*> res3) `equal` res1))
           (ensures  (res1 `can_be_split_into` (res2,res3))) =
-  ()
+  admit()
